add let expressions

src/Pipit.Check.Example.TacX.fst
@@ -86,16 +86,36 @@ let example_GA_GAB_FB_ok (): Lemma (ensures base_case' example_FA_GAB__FB) =
   assert (step_case' example_FA_GAB__FB) by tac_nbe ()
 
 
+let example_let =
+  osystem_of_exp (
+    let open Ck in
+    let open Pipit.Exp.Base in
+    XLet (once (XVar 0)) (
+        let oa = XVar 0 in
+        let a = XVar 1 in
+        oa => once a))
+    1
+
+let example_let' (): Lemma (ensures base_case' example_let) =
+  assert (base_case' example_let) by (tac_base (); T.dump "asdf");
+  assert (step_case' example_let) by tac_nbe ()
+
 let example_requires_invariant =
   osystem_of_exp (
     let open Ck in
-    let a = x0 in
-    let b = x1 in
-    let c = x2 in
-    (once a => (once a => once b) => (once b => once c) => once c))
+    let open Pipit.Exp.Base in
+    // a = 2 + 0
+    XLet (once (XVar 2)) (
+      // b = 1 + 1
+      XLet (once (XVar 2)) (
+        // c = 0 + 2
+        XLet (once (XVar 2)) (
+            let oc = XVar 0 in
+            let ob = XVar 1 in
+            let oa = XVar 2 in
+            (oa /\ (oa => ob) /\ (ob => oc)) => oc))))
     3
 
-[@@expect_failure]
 let example_requires_invariant' (): Lemma (ensures base_case' example_requires_invariant) =
-  assert (base_case' example_requires_invariant) by (tac_base (); T.dump "asdf")
-  // assert (step_case' example_requires_invariant) by tac_nbe ()
+  assert (base_case' example_requires_invariant) by tac_nbe ();
+  assert (step_case' example_requires_invariant) by tac_nbe ()
