src/Pipit.Exp.Base.fst
@@ -1,7 +1,7 @@
 module Pipit.Exp.Base
 
 type prim2 =
-  | And | Or | NAnd | Implies | Eq // | ...
+  | And | Or | Implies | Eq // | ...
 
 let value  = bool
 let var    = nat
@@ -10,7 +10,7 @@ let eval_prim2 (p: prim2) (v1 : value) (v2: value) =
   match p with
   | And  -> v1 && v2
   | Or   -> v1 || v2
-  | Implies -> not v1 || v2
+  | Implies -> if v1 then v2 else true
   | Eq -> v1 = v2
 
 type exp =
@@ -26,6 +26,8 @@ type exp =
   | XThen  : exp -> exp -> exp
   // µx. e[x]
   | XMu    : exp -> exp
+  // let x = e in e[x]
+  | XLet   : exp -> exp -> exp
 
 let xpre_init: value = true
 
@@ -37,6 +39,7 @@ match e with
 | XPre e1 -> wf e1 n
 | XThen e1 e2 -> wf e1 n /\ wf e2 n
 | XMu e1 -> wf e1 (n + 1)
+| XLet e1 e2 -> wf e1 n /\ wf e2 (n + 1)
 
 (* Properties *)
 let rec wf_weaken (e: exp) (n: var) (n': var { n <= n' }):
@@ -54,3 +57,6 @@ let rec wf_weaken (e: exp) (n: var) (n': var { n <= n' }):
     wf_weaken e2 n n'
   | XMu e1 ->
     wf_weaken e1 (n + 1) (n' + 1)
+  | XLet e1 e2 ->
+    wf_weaken e1 n n';
+    wf_weaken e2 (n + 1) (n' + 1)
