src/Pipit.Exp.Subst.fst
@@ -18,6 +18,8 @@ let rec lift (e: exp) (above: var) : exp =
     XThen (lift e1 above) (lift e2 above)
   | XMu e ->
     XMu (lift e (above + 1))
+  | XLet e1 e2 ->
+    XLet (lift e1 above) (lift e2 (above + 1))
 
 (* Substitution *)
 let rec subst (e: exp) (x: var) (payload: exp) : exp =
@@ -37,6 +39,8 @@ let rec subst (e: exp) (x: var) (payload: exp) : exp =
     XThen (subst e1 x payload) (subst e2 x payload)
   | XMu e ->
     XMu (subst e (x + 1) (lift payload 0))
+  | XLet e1 e2 ->
+    XLet (subst e1 x payload) (subst e2 (x + 1) (lift payload 0))
 
 (* Properties *)
 let rec lift_preserves_wf (e: exp) (n x: var):
@@ -53,6 +57,9 @@ let rec lift_preserves_wf (e: exp) (n x: var):
    lift_preserves_wf e1 n x;
    lift_preserves_wf e2 n x
  | XMu e1 -> lift_preserves_wf e1 (n + 1) (x + 1)
+ | XLet e1 e2 ->
+   lift_preserves_wf e1 n x;
+   lift_preserves_wf e2 (n + 1) (x + 1)
 
 let rec subst_preserves_wf (e p: exp) (n: var) (x: var { x < n + 1 }):
   Lemma (requires wf e (n + 1) /\ wf p n)
@@ -70,6 +77,10 @@ let rec subst_preserves_wf (e p: exp) (n: var) (x: var { x < n + 1 }):
   | XMu e1 ->
     lift_preserves_wf p n 0;
     subst_preserves_wf e1 (lift p 0) (n + 1) (x + 1)
+  | XLet e1 e2 ->
+    lift_preserves_wf p n 0;
+    subst_preserves_wf e1 p n x;
+    subst_preserves_wf e2 (lift p 0) (n + 1) (x + 1)
 
 let rec lift_lift_commute (e: exp) (x1: var) (x2: var { x2 <= x1 }):
   Lemma (ensures lift (lift e x1) x2 == lift (lift e x2) (x1 + 1)) =
@@ -85,6 +96,9 @@ let rec lift_lift_commute (e: exp) (x1: var) (x2: var { x2 <= x1 }):
     lift_lift_commute e2 x1 x2
   | XMu e1 ->
     lift_lift_commute e1 (x1 + 1) (x2 + 1)
+  | XLet e1 e2 ->
+    lift_lift_commute e1 x1 x2;
+    lift_lift_commute e2 (x1 + 1) (x2 + 1)
 
 let rec subst_lift_id (e p: exp) (x: var):
   Lemma (ensures subst (lift e x) x p == e) =
@@ -100,6 +114,9 @@ let rec subst_lift_id (e p: exp) (x: var):
     subst_lift_id e2 p x
   | XMu e1 ->
     subst_lift_id e1 (lift p 0) (x + 1)
+  | XLet e1 e2 ->
+    subst_lift_id e1 p x;
+    subst_lift_id e2 (lift p 0) (x + 1)
 
 let rec lift_subst_distribute_le (e p: exp) (x1: var) (x2: var { x2 <= x1 }):
   Lemma (ensures lift (subst e x1 p) x2 == subst (lift e x2) (x1 + 1) (lift p x2)) =
@@ -115,6 +132,10 @@ let rec lift_subst_distribute_le (e p: exp) (x1: var) (x2: var { x2 <= x1 }):
     lift_subst_distribute_le e2 p x1 x2
   | XMu e1 ->
     lift_subst_distribute_le e1 (lift p 0) (x1 + 1) (x2 + 1);
+    lift_lift_commute p x2 0
+  | XLet e1 e2 ->
+    lift_subst_distribute_le e1 p x1 x2;
+    lift_subst_distribute_le e2 (lift p 0) (x1 + 1) (x2 + 1);
     lift_lift_commute p x2 0
 
 let rec subst_subst_distribute_le (e p1 p2: exp) (x1: var) (x2: var { x1 <= x2 }):
@@ -135,6 +156,11 @@ let rec subst_subst_distribute_le (e p1 p2: exp) (x1: var) (x2: var { x1 <= x2 }
     subst_subst_distribute_le e2 p1 p2 x1 x2
   | XMu e1 ->
     subst_subst_distribute_le e1 (lift p1 0) (lift p2 0) (x1 + 1) (x2 + 1);
+    lift_lift_commute p2 x1 0;
+    lift_subst_distribute_le p1 p2 x2 0
+  | XLet e1 e2 ->
+    subst_subst_distribute_le e1 p1 p2 x1 x2;
+    subst_subst_distribute_le e2 (lift p1 0) (lift p2 0) (x1 + 1) (x2 + 1);
     lift_lift_commute p2 x1 0;
     lift_subst_distribute_le p1 p2 x2 0
 
